formal/inference/Code_Generation.thy
@@ -447,6 +447,7 @@ export_code
   try_heuristics aexp_type_check learn finfun_apply infer_types nondeterministic input_updates_register
   (* Scoring functions *)
   naive_score naive_score_eq naive_score_outputs naive_score_comprehensive naive_score_comprehensive_eq_high
+  origin_states
   (* Heuristics *)
   statewise_drop_inputs drop_inputs same_register insert_increment_2 heuristic_1 transitionwise_drop_inputs
   (* Nondeterminism metrics *)
