formal/inference/SelectionStrategies.thy
@@ -51,4 +51,12 @@ definition naive_score_comprehensive_eq_high :: strategy where
                                                else 0
                                              else 0)"
 
+(* Orders by the origin state so we should get zipping down the PTA *)
+definition origin_states :: strategy where
+  "origin_states t1ID t2ID e = (let
+    t1Orig = origin t1ID e;
+    t2Orig = origin t2ID e in
+    if t1Orig = t2Orig \<and> naive_score t1ID t2ID e > 0 then 1000 else
+    naive_score_comprehensive_eq_high t1ID t2ID e)"
+
 end
